<?xml version='1.0'?>
<!DOCTYPE uridef [
	<!ENTITY rdf 		"http://www.w3.org/1999/02/22-rdf-syntax-ns">
	<!ENTITY rdfs 		"http://www.w3.org/2000/01/rdf-schema">
	<!ENTITY owl 		"http://www.w3.org/2002/07/owl">
	<!ENTITY xsd 		"http://www.w3.org/2001/XMLSchema">
	<!ENTITY service 	"http://www.daml.org/services/owl-s/1.1/Service.owl">
	<!ENTITY dc			"http://purl.org/dc/elements/1.1.owl">
	<!ENTITY nextRes	"http://www.ifi.unizh.ch/ddis/ont/next/model/MO_NextResourceModel.owl">	
	<!ENTITY nextGeneral "http://www.ifi.unizh.ch/ddis/ont/next/model/MO_NextGeneralModel.owl">
	<!ENTITY nextProc   "http://www.ifi.unizh.ch/ddis/ont/next/model/MO_NextProcessModel.owl">	
	<!ENTITY nextAuthors "http://www.ifi.unizh.ch/ddis/ont/next/model/instances/MI_NextAuthors.owl">
]>

<rdf:RDF
	xmlns:rdf =		"&rdf;#" 
	xmlns:rdfs =	"&rdfs;#" 
	xmlns:owl =		"&owl;#" 
	xmlns:xsd =		"&xsd;#" 
	xmlns:service = "&service;#"  
	xmlns:dc=	    "&dc;#"	
	xmlns:nextProc= "&nextProc;#"
	xmlns:nextRes=	"&nextRes;#"
	xmlns:nextGeneral="&nextGeneral;#"
	xmlns:nextAuthors="&nextAuthors;#"	
	xml:base=		"http://www.ifi.unizh.ch/ddis/ont/next/model/NextCaseModel.owl"
> 
	<owl:Ontology rdf:ID="NextCaseModel">
		<rdfs:comment>Upper-Level Ontology for NExT project Model.</rdfs:comment>
		<owl:versionInfo>MO_NextProjectModel.owl v1.2, 2006-03-06</owl:versionInfo> 
		<dc:creator>Michael Daenzer</dc:creator>
		<dc:contributor>Konstantin Pervushin</dc:contributor>
		<dc:contributor>Peter Vorburger</dc:contributor>
		<dc:contributor>Abraham Bernstein</dc:contributor>
		<dc:date>2006-03-06</dc:date>
		<dc:rights>copyright 2006 by Michael Daenzer, University of Zurich</dc:rights> 
		
		<owl:imports rdf:resource="http://www.ifi.unizh.ch/ddis/ont/next/model/MO_NextResourceModel.owl"/>
		<owl:imports rdf:resource="http://www.ifi.unizh.ch/ddis/ont/next/model/MO_NextGeneralModel.owl"/>
		<owl:imports rdf:resource="http://www.ifi.unizh.ch/ddis/ont/next/model/instances/MI_NextAuthors.owl"/>	
		<owl:imports rdf:resource="http://www.ifi.unizh.ch/ddis/ont/next/model/MO_NextProcessModel.owl"/>
	</owl:Ontology>
	
	<owl:Class rdf:ID="NExTProject">
		<rdfs:comment>The class for a NExT project. This may be subclassed with a domain-specific project class</rdfs:comment>		
		<rdfs:subClassOf>
	    	<owl:Restriction>
		      <owl:onProperty rdf:resource="#hasPlan"/>
		      <owl:cardinality rdf:datatype="&xsd;#nonNegativeInteger">1</owl:cardinality>  
			</owl:Restriction>
	   </rdfs:subClassOf>	
		<rdfs:subClassOf>
	    	<owl:Restriction>
		      <owl:onProperty rdf:resource="#hasProcessPath"/>
		      <owl:cardinality rdf:datatype="&xsd;#nonNegativeInteger">1</owl:cardinality>  
			</owl:Restriction>
	   </rdfs:subClassOf>
		<rdfs:subClassOf>
	    	<owl:Restriction>
		      <owl:onProperty rdf:resource="#hasValueList"/>
		      <owl:cardinality rdf:datatype="&xsd;#nonNegativeInteger">1</owl:cardinality>  
			</owl:Restriction>
	   </rdfs:subClassOf>		
	</owl:Class>
	
	<owl:ObjectProperty rdf:ID="hasPlan">
		<rdfs:comment>relates a NExT project with its process plan</rdfs:comment>
		<rdfs:domain rdf:resource="#NExTProject"/>
		<rdfs:range rdf:resource="#ProcessPlan"/>
	</owl:ObjectProperty>
	
	<owl:Class rdf:ID="ProcessPlan">
		<rdfs:comment>A Next process representing the process plan of a NExT project</rdfs:comment>
		<rdfs:subClassOf rdf:resource="&nextProc;#NextProcess"/>	
	</owl:Class>
	
	<owl:Class rdf:ID="ProcessPath">
		<rdfs:comment>a temporally ordered list of executed processes through the process plan</rdfs:comment>
		<rdfs:subClassOf rdf:resource="&rdf;#List"/>
	</owl:Class>
	
	<owl:ObjectProperty rdf:ID="hasPathway">
		<rdfs:comment>relates a NExT project with the pathway trough the process plan</rdfs:comment>
		<rdfs:domain rdf:resource="#NExTProject"/>
		<rdfs:range rdf:resource="#ProcessPath"/>
	</owl:ObjectProperty>
	
	<owl:Class rdf:ID="ValueList">
		<rdfs:comment>the temporally ordered list of data values changes throughout the pathway through the process plan</rdfs:comment>
		<rdfs:subClassOf rdf:resource="&rdf;#List"/>
	</owl:Class>
	
	<owl:ObjectProperty rdf:ID="hasValueList">
		<rdfs:comment>relates a NExT project with the history of the values iof its data</rdfs:comment>
		<rdfs:domain rdf:resource="#NExTProject"/>
		<rdfs:range rdf:resource="#ValueList"/>
	</owl:ObjectProperty>
</rdf:RDF>